reduction to fSAT, apart from a few minor technical lemmas

theories/L/Complexity/Cook/BinaryPR_to_FSAT.v
@@ -19,6 +19,7 @@ Section fixInstance.
   Notation final := (final bpr).
   Notation steps := (steps bpr). 
 
+  Context (A : BinaryPR_wellformed bpr). 
   Notation llength := (length init). 
 
   Implicit Types (a : assgn) (v : var). 
@@ -34,39 +35,55 @@ Section fixInstance.
     | a :: l => a ∧ listAnd l
     end.  
 
-  (*generate the list of values assigned to the variables in range [lower, upper) *)
-  Fixpoint explicitAssignment a lower upper := 
-    match upper with 0 => [] 
-        | S upper => if upper <? lower then [] 
-              else explicitAssignment a lower upper ++ [list_in_decb Nat.eqb a upper]
-        end. 
+  (*generate the list of values assigned to the variables in range [lower, lower + len) *)
+  Fixpoint explicitAssignment a lower len := 
+    match len with
+      | 0 => [] 
+      | S len => explicitAssignment a lower len ++ [list_in_decb Nat.eqb a (lower + len)]
+    end. 
 
-  Lemma explicitAssignment_length a lower upper : |explicitAssignment a lower upper| = upper - lower. 
+
+  Lemma explicitAssignment_length a lower len : |explicitAssignment a lower len| = len. 
   Proof. 
-    revert lower. induction upper; intros. 
-    - cbn. destruct lower; now cbn. 
-    - destruct lower. 
-      + rewrite app_length, IHupper. cbn. lia. 
-      + cbn. 
-        destruct Nat.leb eqn:H1.
-        * apply Nat.leb_le in H1. cbn. lia. 
-        * rewrite app_length. rewrite IHupper. cbn. apply Nat.leb_nle in H1. lia. 
+    revert lower. induction len; intros; cbn. 
+    - reflexivity. 
+    - rewrite app_length, IHlen. now cbn.
   Qed. 
 
-  Lemma explicitAssignment_nth a lower upper k : 
-     k < upper - lower -> nth_error (explicitAssignment a lower upper) k = Some (evalVar a (lower + k)). 
+  Lemma explicitAssignment_nth a lower len k : 
+     k < len -> nth_error (explicitAssignment a lower len) k = Some (evalVar a (lower + k)). 
   Proof. 
-    intros. induction upper. 
+    intros. induction len. 
     - lia. 
-    - unfold explicitAssignment. assert (not (upper < lower)) by (intros; lia). 
-      rewrite (proj2 (Nat.ltb_nlt _ _) H0 ). 
-      fold explicitAssignment. 
-      destruct (le_lt_dec (upper - lower) k).
-      + assert (upper - lower = k) as <- by lia.
-        rewrite nth_error_app2; rewrite explicitAssignment_length; [ rewrite Nat.sub_diag; cbn | lia].  
-        unfold evalVar. enough (upper = lower + (upper - lower)) by easy. lia.  
-      + rewrite nth_error_app1; [ | rewrite explicitAssignment_length; easy ]. now apply IHupper. 
+    - cbn. destruct (le_lt_dec len k).
+      + assert (len = k) as <- by lia.
+        rewrite nth_error_app2; rewrite explicitAssignment_length; [ rewrite Nat.sub_diag; cbn | lia]. easy.
+      + rewrite nth_error_app1; [ | rewrite explicitAssignment_length; easy ]. now apply IHlen. 
   Qed. 
+
+  Lemma explicitAssignment_lenO a s l : explicitAssignment a s l = [] <-> l = 0. 
+  Proof. 
+    specialize (explicitAssignment_length a s l). 
+    split; intros. 
+    - rewrite H0 in H. easy. 
+    - subst. destruct explicitAssignment; cbn in *; congruence. 
+  Qed. 
+
+  Corollary explicitAssignment_lenO' a l : explicitAssignment a l 0 = []. 
+  Proof. 
+    apply explicitAssignment_lenO. easy.
+  Qed. 
+
+  Lemma explicitAssignment_app a l1 len1 len2: explicitAssignment a l1 (len1 + len2) = explicitAssignment a l1 len1 ++ explicitAssignment a (l1 + len1) len2. 
+  Proof. 
+    induction len2; cbn. 
+    - now rewrite Nat.add_0_r, app_nil_r. 
+    - rewrite Nat.add_succ_r. cbn. rewrite IHlen2, app_assoc. easy. 
+  Qed. 
+
+  Lemma explicitAssignment_length' a n: |explicitAssignment a 0 n| = n.
+  Proof. rewrite explicitAssignment_length. lia. Qed. 
+
 
   Inductive varsInRange (min max : nat) : formula -> Prop := 
     | varsInRangeTrue : varsInRange min max Ftrue
@@ -84,9 +101,35 @@ Section fixInstance.
   Definition predicate := list bool -> Prop. 
   Implicit Type (p : predicate).
   Definition encodesPredicateAt (start : nat) (l : nat) f p:= 
-    varsInRange start (l + start) f /\ forall a, satisfies a f <-> p (explicitAssignment a start (l + start)). 
+    varsInRange start (l + start) f /\ forall a, satisfies a f <-> p (explicitAssignment a start l). 
 
   Definition projVars start len (l : list bool) := firstn len (skipn start l). 
+
+  Lemma projVars_length l s m : |l| >= (s + m) -> |projVars s m l| = m. 
+  Proof. 
+    intros. unfold projVars. rewrite firstn_length. rewrite skipn_length. lia. 
+  Qed. 
+
+  Lemma projVars_app1 l1 l2 m : |l1| = m -> projVars 0 m (l1 ++ l2) = l1.
+  Proof. 
+    intros. unfold projVars. cbn. rewrite firstn_app. subst. 
+    now rewrite Nat.sub_diag, firstn_O, app_nil_r, firstn_all.
+  Qed. 
+
+  Lemma projVars_app2 l1 l2 u m : |l1| = u -> projVars u m (l1 ++ l2) = projVars 0 m l2. 
+  Proof. 
+    intros. unfold projVars. rewrite skipn_app; [ | easy]. now cbn. 
+  Qed. 
+
+  Lemma projVars_app3 l1 l2 u1 u2 m : |l1| = u1 -> projVars (u1 + u2) m (l1 ++ l2) = projVars u2 m l2. 
+  Proof. 
+    intros. unfold projVars. erewrite skipn_add; [ easy| lia]. 
+  Qed. 
+
+  Lemma projVars_all l m : m = |l| -> projVars 0 m l = l. 
+  Proof.
+    intros. unfold projVars. cbn. rewrite H. apply firstn_all. 
+  Qed. 
 
   (*encodings of two predicates can be combined*)
   Definition combinedLength start1 start2 l1 l2 := max (start1 +l1) (start2 + l2) - min start1 start2. 
@@ -121,19 +164,18 @@ Section fixInstance.
     - destruct l; cbn; [ now destruct k | apply IHm]. 
   Qed. 
 
-  Lemma projVars_combined1 s1 s2 l1 l2 a: explicitAssignment a s1 (l1 + s1) = projVars (s1 - combinedStart s1 s2) l1 (explicitAssignment a (combinedStart s1 s2) (combinedLength s1 s2 l1 l2 + combinedStart s1 s2)).
+  Lemma projVars_combined1 s1 s2 l1 l2 a: explicitAssignment a s1 l1 = projVars (s1 - combinedStart s1 s2) l1 (explicitAssignment a (combinedStart s1 s2) (combinedLength s1 s2 l1 l2)).
   Proof. 
     unfold projVars. 
     apply list_eq_nth_error. split. 
     - rewrite explicitAssignment_length. unfold combinedStart, combinedLength. rewrite firstn_length. 
       rewrite skipn_length. rewrite explicitAssignment_length. lia. 
-    - intros. rewrite explicitAssignment_length, Nat.add_sub in H. unfold combinedStart, combinedLength. 
-      rewrite Nat.sub_add; [ | lia]. 
+    - intros. rewrite explicitAssignment_length in H. unfold combinedStart, combinedLength. 
       rewrite nth_error_firstn; [ | apply H].  
       rewrite nth_error_skipn. rewrite !explicitAssignment_nth; [easy | lia | lia]. 
   Qed. 
 
-  Lemma projVars_combined2 s1 s2 l1 l2 a: explicitAssignment a s2 (l2 + s2) = projVars (s2 - combinedStart s1 s2) l2 (explicitAssignment a (combinedStart s1 s2) (combinedLength s1 s2 l1 l2 + combinedStart s1 s2)). 
+  Lemma projVars_combined2 s1 s2 l1 l2 a: explicitAssignment a s2 l2 = projVars (s2 - combinedStart s1 s2) l2 (explicitAssignment a (combinedStart s1 s2) (combinedLength s1 s2 l1 l2)). 
   Proof. 
     unfold combinedStart, combinedLength. rewrite Nat.min_comm. rewrite Nat.max_comm. apply projVars_combined1. 
   Qed. 
@@ -189,13 +231,13 @@ Section fixInstance.
     split. 
     - apply encodeLiteral_varsInRange. 
     - intros. split; intros. 
-      + apply encodeLiteral_correct in H. specialize (explicitAssignment_length a v (S v)) as H1. 
-        replace (S v - v) with 1 in H1 by lia. assert (0 < S v - v) as H2 by lia. 
-        specialize (@explicitAssignment_nth a v (S v) 0 H2) as H3. 
+      + apply encodeLiteral_correct in H. specialize (explicitAssignment_length a v 1) as H1. 
+        assert (0 < 1) as H2 by lia. 
+        specialize (@explicitAssignment_nth a v 1 0 H2) as H3. 
         destruct explicitAssignment as [ | s l]; cbn in H1; [ congruence | destruct l; [ | cbn in H1; congruence]]. 
         cbn in H3. now inv H3. 
-      + apply encodeLiteral_correct.  assert (0 < S v - v) as H2 by lia.
-        specialize (@explicitAssignment_nth a v (S v) 0 H2) as H1. 
+      + apply encodeLiteral_correct. assert (0 < 1) as H2 by lia.
+        specialize (@explicitAssignment_nth a v 1 0 H2) as H1. 
         rewrite H in H1; cbn in H1. now inv H1. 
   Qed. 
 
@@ -224,7 +266,7 @@ Section fixInstance.
     revert start. induction l; intros. 
     - cbn. split; [eauto | ]. unfold satisfies.  
       intros; split. 
-      + intros _. destruct start; cbn; [easy | rewrite Nat.leb_refl; easy]. 
+      + intros _. destruct start; now cbn. 
       + intros _. easy. 
     - cbn. specialize (@encodesPredicate_and start (S start) 1 (|l|) (encodeLiteral start a) (encodeListAt (S start) l) _ _ (encodeLiteral_encodesPredicate start a) (IHl (S start))) as H1.
       replace (combinedStart start (S start)) with (start) in H1 by (unfold combinedStart; lia). 
@@ -239,17 +281,83 @@ Section fixInstance.
         now apply firstn_all_inv. 
   Qed. 
 
+  Ltac encodesPredicateAt_comp_simp H := 
+    unfold combinedStart, combinedLength in H;
+    try (rewrite Nat.min_l in H by nia); try (rewrite Nat.min_r in H by nia);
+    try (rewrite Nat.max_l in H by nia); try (rewrite Nat.max_r in H by nia);
+    try rewrite !Nat.sub_diag in H; cbn -[projVars] in H.
+
   (*encoding of windows *)
   Definition encodeWindowAt (startA startB : nat) (win : PRWin bool) := encodeListAt startA (prem win) ∧ encodeListAt startB (conc win). 
-  Lemma encodeWindowAt_encodesPredicate start win : encodesPredicateAt start (llength + offset) (encodeWindowAt start (start + llength) win) (fun m => firstn offset m = prem win /\ skipn llength m = conc win). 
+  Lemma encodeWindowAt_encodesPredicate start len win : win el windows -> encodesPredicateAt start (len + width) (encodeWindowAt start (start + len) win) (fun m => projVars 0 width m = prem win /\ projVars len width m = conc win /\ |m| = len + width). 
   Proof. 
-  Admitted. 
+    intros H0. 
+    specialize (encodesPredicate_and (encodeListAt_encodesPredicate start (prem win)) (encodeListAt_encodesPredicate (start + len) (conc win))) as H. 
+    destruct A as (_ & _ & _ & A0 & A1 & _). apply A1 in H0 as (H0 & H0').
+    encodesPredicateAt_comp_simp H. 
+    rewrite !H0 in H. rewrite !H0' in H.
+    replace (start + len + width - start) with (len + width) in H by lia. 
+    replace (start + len - start) with len in H by lia.
+    unfold encodeWindowAt. eapply encodesPredicateAt_extensional; [ | apply H].
+    tauto.
+  Qed.
 
   Definition encodeWindowsAt (startA startB : nat) := listOr (map (encodeWindowAt startA startB) windows). 
 
-  Lemma encodeWindowsAt_encodesPredicate start : encodesPredicateAt start (llength + offset) (encodeWindowsAt start (start + llength)) (fun m => exists win, win el windows /\ firstn offset m = prem win /\ skipn llength m = conc win). 
+  Lemma skipn_firstn_shift (X : Type) (m : list X) len l : skipn l (firstn len m) = firstn (len - l) (skipn l m). 
   Proof. 
-  Admitted. 
+    revert l len. induction m; cbn; intros. 
+    - rewrite !firstn_nil, !skipn_nil, firstn_nil. easy. 
+    - destruct len. 
+      + cbn. now destruct l.
+      + cbn. destruct l; cbn; [ easy | ]. now rewrite IHm. 
+  Qed. 
+
+  Lemma skipn_skipn (X : Type) (m : list X) l1 l2 : skipn l1 (skipn l2 m) = skipn (l1 + l2) m. 
+  Proof. 
+    revert l1 l2. 
+    induction m; intros; destruct l2; cbn; try now rewrite !skipn_nil. 
+    - now rewrite Nat.add_0_r. 
+    - rewrite IHm. rewrite Nat.add_succ_r. easy. 
+  Qed. 
+
+  Lemma skipn_firstn_skipn (X : Type) (m : list X) l1 l2 len2 : 
+    skipn l1 (firstn len2 (skipn l2 m)) = firstn (len2 - l1) (skipn (l1 + l2) m). 
+  Proof. 
+    intros. 
+    rewrite skipn_firstn_shift. now rewrite skipn_skipn. 
+  Qed. 
+
+  Lemma projVars_comp l1 l2 len1 len2 m: projVars l1 len1 (projVars l2 len2 m) = projVars (l1 + l2) (min len1 (len2 - l1)) m. 
+  Proof. 
+    unfold projVars. intros. 
+    rewrite skipn_firstn_skipn. rewrite firstn_firstn. reflexivity. 
+  Qed. 
+
+  Lemma encodeWindowsAt_encodesPredicate len start : len >= width -> encodesPredicateAt start (len + width) (encodeWindowsAt start (start + len)) (fun m => exists win, win el windows /\ projVars 0 width m = prem win /\ projVars len width m = conc win /\ |m| = len + width). 
+  Proof. 
+    intros F0.
+    specialize (encodeWindowAt_encodesPredicate) as H1. 
+    unfold encodeWindowsAt. 
+    induction windows. 
+    - cbn. split. 
+      + eauto. 
+      + intros; split. 
+        * unfold satisfies. cbn. congruence. 
+        * intros (win & [] & _). 
+    - cbn. match type of IHl with ?a -> _ => assert a as H by (intros; apply H1; eauto); apply IHl in H; clear IHl end. 
+      specialize (H1 start len a (or_introl eq_refl)). 
+      specialize (encodesPredicate_or H1 H) as H2. clear H1 H. 
+      cbn in H2. 
+      destruct A as (_ & _ & (k & A1 & A2) & _).
+      encodesPredicateAt_comp_simp H2. 
+      replace (start + (len + width) - start) with (len + width) in H2 by lia.
+      eapply encodesPredicateAt_extensional; [ | apply H2]. 
+      intros; cbn. 
+      rewrite !projVars_comp. cbn. rewrite !Nat.min_l by lia. rewrite Nat.add_0_r. split; intros. 
+      + destruct H as (win & [<- | H] & F1 & F2 & F3); (rewrite projVars_length; [ split; [ | easy] | easy]); [now left | right; eauto].
+      + destruct H as ([(F1 & F2 & F3) | (win & H & F1 & F2 & F3)] & F4); eauto 7. 
+  Qed. 
 
   (*we only need to place a window every offset fields, but subtracting offset isn't structurally recursive *)
   (*therefore we use a stepindex (initalise to the same value as l) *)
@@ -260,50 +368,420 @@ Section fixInstance.
                     | S stepindex => encodeWindowsAt startA startB ∧ encodeWindowsInLine' stepindex (l - offset) (startA + offset) (startB + offset)
                     end.
 
-  (*TODO: need the additional constraint that variables do not overlap *)
-  (*Lemma encodeWindowsInLine'_correct (l : nat) (startA startB : nat) :*)
-    (*l >= width -> *)
-    (*forall a, satisfies a (encodeWindowsInLine' l startA startB) <-> valid offset width windows (explicitAssignment a startA (startA + l)) (explicitAssignment a startB (startB + l)). *)
-  (*Proof. *)
-  (*Admitted. *)
- 
-  Definition encodeWindowsInLine start := encodeWindowsInLine' llength llength start (start + llength). 
-  Lemma encodeWindowsInLine_encodesPredicate start : encodesPredicateAt start (llength + llength) (encodeWindowsInLine start) (fun m => valid offset width windows (firstn llength m) (skipn llength m)). 
+  Lemma encodeWindowsInLine'_stepindex_monotone index index' startA startB : index' >= index -> encodeWindowsInLine' index index startA startB = encodeWindowsInLine' index' index startA startB. 
   Proof. 
+    intros. 
+    destruct A as (A1 & _).
+    revert index' H.  induction index; intros. 
+    - cbn. destruct index'; cbn; (destruct width; [ lia | easy]).
+    - destruct index'; [lia | ]. apply le_S_n in H. apply IHindex in H. 
+      cbn. 
   Admitted.
 
-  Fixpoint encodeAllLines' (t : nat) (start : nat) := 
+  SearchAbout firstn.
+  Lemma firstn_add (X : Type) (m : list X) l1 l2 : firstn (l1 + l2) m = firstn l1 m ++ firstn l2 (skipn l1 m). 
+  Proof. 
+    revert l1 l2. induction m; intros. 
+    - now rewrite !skipn_nil, !firstn_nil.
+    - destruct l1; cbn; [ easy | ]. now rewrite IHm. 
+  Qed. 
+
+  Lemma projVars_add s l1 l2 m : projVars s (l1 + l2) m = projVars s l1 m ++ projVars (s + l1) l2 m. 
+  Proof. 
+    unfold projVars. rewrite firstn_add, skipn_skipn. now rewrite Nat.add_comm. 
+  Qed.
+
+  Lemma encodeWindowsInLine'_encodesPredicate start l : l <= llength -> (exists k, l = k * offset) -> encodesPredicateAt start (l + llength) (encodeWindowsInLine' l l start (start + llength)) (fun m => valid offset width windows (projVars 0 l m) (projVars llength l m) /\ |m| = l + llength). 
+  Proof. 
+    intros A0.
+    (*need strong induction *)
+    destruct A as (A1 & A4 & A2 & A5 & A7 & A3). 
+    revert start A0.  
+    apply complete_induction with (x := l). clear l. intros l IH. intros. 
+
+    destruct l.
+    - cbn. destruct width; [ lia | ]. split; [eauto | ]. 
+      intros a. split; [ intros; split; [constructor | ] | intros _; unfold satisfies; eauto]. now rewrite explicitAssignment_length. 
+    - destruct (le_lt_dec width (S l)). 
+      + assert (~ (S l) < width) as H3%Nat.ltb_nlt by lia. cbn -[projVars]; setoid_rewrite H3. 
+        destruct offset as [ | offset]; [ lia | ].
+        (* we use the IH for l - offset *)
+ 
+        assert (S l - S offset < S l) as H1 by lia. apply IH with (start := start + S offset) in H1. 2: nia. 
+        2: { destruct H as (k & H). destruct k; [ lia | ]. exists k. lia. }
+        clear H IH. 
+        assert (llength >= width) as H0 by lia.
+        apply (encodeWindowsAt_encodesPredicate start) in H0. 
+        specialize (encodesPredicate_and H0 H1) as H2. clear H1 H0.
+        encodesPredicateAt_comp_simp H2. 
+        replace (start + S offset + llength) with (start + llength + S offset) in H2 by lia. 
+        replace (start + S offset + (l - offset + llength) - start) with (S (l + llength)) in H2. 
+        2: { destruct A2 as (? & A2 & A6). nia. }
+        
+        rewrite encodeWindowsInLine'_stepindex_monotone with (index' := l) in H2; [ | lia].
+        eapply encodesPredicateAt_extensional; [ | apply H2].
+        clear H2 H3. 
+        intros. 
+        destruct A2 as (k & A2 & A2').
+        assert (S l = S offset + (S l - S offset)) as H by nia.  
+        split; intros. 
+        * destruct H0 as (H1 & H2). rewrite projVars_length; [ | easy]. 
+          rewrite H in H1. clear H. 
+          rewrite !projVars_add in H1. inv H1.
+          2 : { exfalso. apply list_eq_length in H. rewrite !app_length in H. rewrite !projVars_length in H; [ | easy | easy]. nia. }
+          1: { exfalso. apply list_eq_length in H0. rewrite !app_length in H0. rewrite projVars_length in H0; [ | cbn; nia]. cbn in H0. lia. } 
+
+          apply app_eq_length in H as (-> & ->); [ | rewrite projVars_length; [easy | nia] ].
+          apply app_eq_length in H0 as (-> & ->); [ | rewrite projVars_length; [easy | nia]]. 
+          specialize (@projVars_length m 0 (S l)) as H8.
+          rewrite projVars_length; [ | nia]. split; [ split; [ | split; [ | easy]] | easy]; clear H8.
+          -- exists win. rewrite !projVars_comp; cbn. rewrite !Nat.min_l by lia. 
+             rewrite !Nat.add_0_r.
+             clear H3 H4 H5. rewrite <- !projVars_add in H7. 
+             replace (S offset + (l - offset)) with (width + (S l - width)) in H7 by nia. 
+             rewrite !projVars_add in H7.
+             split; [ easy | split; [ | split; [ | easy]]]; apply A7 in H6 as (H6 & H6'). 
+             ++ destruct H7 as ((b & H7) & _). eapply app_eq_length in H7; [ easy| rewrite projVars_length; easy ]. 
+             ++ destruct H7 as (_ & (b & H7)). eapply app_eq_length in H7; [ easy | rewrite projVars_length; easy].
+          -- clear H7 H6. 
+             rewrite projVars_comp. cbn. replace (start + S offset - start) with (S offset) by lia. rewrite Nat.min_l by lia. 
+             rewrite projVars_comp. cbn. rewrite Nat.min_l by lia. 
+             apply H3. 
+        * (*other direction of the equivalence *)
+          destruct H0 as ((H1  & (H2 & H3)) & H4). split; [ | apply H4]. 
+          rewrite H. rewrite !projVars_add. 
+          destruct H1 as (win & H1 & F1 & F2 & _). 
+          econstructor 3. 
+          -- clear H1. rewrite !projVars_comp in H2. rewrite !Nat.min_l in H2 by lia.
+             replace (start + S offset - start) with (S offset) in H2 by lia. 
+             apply H2. 
+          -- rewrite projVars_length; lia. 
+          -- rewrite projVars_length; lia. 
+          -- clear H2. apply H1. 
+          -- clear H2. rewrite <- !projVars_add. 
+             replace (S offset + (S l - S offset)) with (width + (S l - width)) by lia. 
+             rewrite !projVars_add. 
+             rewrite projVars_comp in F1, F2. rewrite !Nat.min_l in F1, F2 by lia. 
+             rewrite Nat.add_0_r in F2; cbn in F1, F2.
+             rewrite F1, F2. split; unfold prefix; eauto. 
+    + (*the case where the remaining string is too short for a rewrite window to hold - validity holds vacuously *)
+      clear IH. assert ( (S l) < width) as H3%Nat.ltb_lt by lia. cbn -[projVars]; setoid_rewrite H3.
+      split; [eauto | ]. unfold satisfies; cbn [evalFormula]. setoid_rewrite explicitAssignment_length. 
+      intros a; split; [intros _ | ]. 
+      * split; [ | easy]. destruct H as (k & H). eapply valid_vacuous. 
+        -- rewrite !projVars_length; [easy | rewrite explicitAssignment_length; lia | rewrite explicitAssignment_length; lia]. 
+        -- rewrite projVars_length; [ easy | rewrite explicitAssignment_length; lia]. 
+        -- rewrite projVars_length; [ | rewrite explicitAssignment_length; lia]. 
+           (*here we need the assumption that l is a multiple of offset *)
+           apply H. 
+      * intros _; easy. 
+  Qed.
+
+  Definition encodeWindowsInLine start := encodeWindowsInLine' llength llength start (start + llength). 
+  Lemma encodeWindowsInLine_encodesPredicate start : encodesPredicateAt start (llength + llength) (encodeWindowsInLine start) (fun m => valid offset width windows (projVars 0 llength m) (projVars llength llength m) /\ |m| = llength + llength). 
+  Proof. 
+    unfold encodeWindowsInLine.
+    apply (@encodeWindowsInLine'_encodesPredicate start llength); [easy | apply A].
+  Qed. 
+
+  Fixpoint encodeWindowsInAllLines' (start : nat) (t : nat)  := 
     match t with 
     | 0 => Ftrue
-    | S t => encodeWindowsInLine start ∧ encodeAllLines' t (start + llength)
+    | S t => encodeWindowsInLine start ∧ encodeWindowsInAllLines' (start + llength) t
     end. 
 
-  Definition encodeAllLines := encodeAllLines' steps 0. 
+  Definition encodeWindowsInAllLines := encodeWindowsInAllLines' 0 steps. 
 
-  Lemma encodeAllLines_encodesPred : encodesPredicateAt 0 (steps * llength) encodeAllLines (fun m => relpower (valid offset width windows) steps (firstn llength m) (skipn ((steps -1) * llength) m)). 
+  Lemma encodeWindowsInAllLines'_encodesPredicate start : encodesPredicateAt start ((S steps) * llength) (encodeWindowsInAllLines' start steps) 
+    (fun m => (forall i, 0 <= i < steps -> valid offset width windows (projVars (i * llength) llength m) (projVars (S i * llength) llength m)) /\ |m| = (S steps) * llength). 
   Proof. 
-  Admitted. 
+    revert start. induction steps; cbn; intros. 
+    - split; [ easy | ]. rewrite !Nat.add_0_r. 
+      intros a; unfold satisfies; cbn; split; [ intros _; split; [intros; lia | rewrite explicitAssignment_length; lia]| easy]. 
+    - specialize (encodeWindowsInLine_encodesPredicate start) as H1. 
+      specialize (IHn (start + llength)). 
+      specialize (encodesPredicate_and H1 IHn) as H. clear IHn H1. 
+      encodesPredicateAt_comp_simp H. 
+      replace (start + llength + S n * llength - start) with (llength + (llength + n * llength)) in H by lia. 
+      replace (start + llength - start) with llength in H by lia. 
+      eapply encodesPredicateAt_extensional; [ | apply H].
+      clear H. intros m. cbn -[projVars]. 
+      rewrite !projVars_comp. setoid_rewrite projVars_comp. cbn. rewrite !Nat.min_l by lia. 
+      rewrite Nat.add_0_r. split. 
+      + intros (H1 & H2). split; [ split |  easy]. 
+        * specialize (H1 0). cbn in H1. rewrite Nat.add_0_r in H1. split; [apply H1; lia | now rewrite projVars_length].
+        * split; [ | now rewrite projVars_length]. intros i H. 
+          specialize (H1 (S i)). cbn in H1. rewrite Nat.add_comm. rewrite <- Nat.add_assoc. 
+          rewrite !Nat.min_l by nia.
+          setoid_rewrite Nat.add_comm at 3.
+          apply H1. lia.
+      + intros ((H1 & (H2 & _)) & H3). split; [ clear H3| apply H3]. intros i H. 
+        destruct i. 
+        * cbn. rewrite Nat.add_0_r. apply H1.
+        * specialize (H2 i). 
+          rewrite !Nat.min_l in H2 by nia.
+          cbn. rewrite Nat.add_comm. rewrite Nat.add_assoc. now apply H2. 
+  Qed.
 
-  Fixpoint encodeSubstringInLine (s : list bool) (l : nat) (start : nat) := 
+  Corollary encodeWindowsInAllLines_encodesPredicate : encodesPredicateAt 0 ((S steps) * llength) encodeWindowsInAllLines 
+    (fun m => (forall i, 0 <= i < steps -> valid offset width windows (projVars (i * llength) llength m) (projVars (S i * llength) llength m)) /\ |m| = (S steps) * llength). 
+  Proof. 
+    unfold encodeWindowsInAllLines. apply encodeWindowsInAllLines'_encodesPredicate. 
+  Qed. 
+
+  Fixpoint encodeSubstringInLine' (s : list bool) (stepindex l : nat) (start : nat) := 
     if l <? |s| then Ffalse
-                else match l with 
-                  | 0 => Ffalse
-                  | S l => encodeListAt start s ∨ encodeSubstringInLine s l (S start) 
-                  end. 
-  Definition encodeFinalConstraint (start : nat) := listOr (map (fun s => encodeSubstringInLine s llength start) final). 
+                  else match stepindex with 
+                    | 0 => (match s with [] => Ftrue | _ => Ffalse end)
+                    | S stepindex => encodeListAt start s ∨ encodeSubstringInLine' s stepindex (l - offset) (start + offset) 
+                    end.
 
-  Lemma encodeFinalConstraint_encodesPredicate start : encodesPredicateAt start llength (encodeFinalConstraint start) (satFinal offset llength final).
+  Lemma encodeSubstringInLine'_stepindex_monotone s index1 index2 start : 
+    index2 >= index1 -> encodeSubstringInLine' s index1 index1 start = encodeSubstringInLine' s index2 index1 start.
   Proof. 
   Admitted. 
 
-  Definition encodeTableau := encodeListAt 0 init ∧ encodeAllLines ∧ encodeFinalConstraint ((steps -1) * llength).
-  Lemma encodeTableau_encodesPredicate : encodesPredicateAt 0 (steps * llength) encodeTableau (fun m => firstn llength m = init /\ relpower (valid offset width windows) steps init (skipn ((steps -1) * llength) m) /\ satFinal offset llength final (skipn ((steps -1) * llength) m)). 
+  Lemma projVars_length_le start l m: |projVars start l m| <= |m|. 
   Proof. 
+    unfold projVars. 
+    rewrite firstn_length. rewrite skipn_length. lia. 
+  Qed. 
+
+  Lemma projVars_length_le2 start l m : |projVars start l m| <= l.
+  Proof. 
+    unfold projVars. rewrite firstn_length, skipn_length. lia. 
+  Qed. 
+
+  Lemma projVars_in_ge start l m : start <= |m| -> projVars start (|l|) m = l -> |m| >= start + |l|. 
+  Proof. 
+    intros H0 H. unfold projVars in H. rewrite <- H, firstn_length, skipn_length. lia.
+  Qed. 
+
+  Lemma encodeSubstringInLine'_encodesPredicate s start l : l <= llength -> (exists k, l = k * offset) -> encodesPredicateAt start l (encodeSubstringInLine' s l l start) (fun m => (exists k, k * offset <= l /\ projVars (k * offset) (|s|) m = s) /\ |m| = l). 
+  Proof. 
+    (*need strong induction *)
+    destruct A as (A1 & A4 & A2 & A5 & A7 & A3). 
+    revert start.  
+    apply complete_induction with (x := l). clear l. intros l IH. intros. 
+
+    destruct l.
+    - cbn -[projVars]. destruct s; cbn -[projVars]. 
+      + (*trivially true *) split; [ easy | intros; unfold satisfies; cbn; split; intros _; eauto].
+        split; [exists 0; split; [lia | easy] | easy ].
+      + (*trivially false *)
+        split; [ easy | ]. intros a; split.
+        * unfold satisfies; cbn; congruence. 
+        * intros ((k & H1 & H2) & _). destruct k; [clear H1 | nia].
+          cbn in H2. congruence. 
+    - destruct (le_lt_dec (|s|) (S l)). 
+      + assert (~ (S l) < (|s|)) as H3%Nat.ltb_nlt by lia. cbn -[projVars]; setoid_rewrite H3. 
+        destruct offset as [ | offset]; [ lia | ].
+        (* we use the IH for l - offset *)
+ 
+        assert (S l - S offset < S l) as H1 by lia. apply IH with (start := start + S offset) in H1. 2: nia. 
+        2: { destruct H0 as (k & H0). destruct k; [ lia | ]. exists k. lia. }
+        clear H IH. 
+        specialize (encodeListAt_encodesPredicate start s) as H2.
+        specialize (encodesPredicate_or H2 H1) as H. clear H1 H2 H3.
+        encodesPredicateAt_comp_simp H.
+        destruct H0 as (k & H0).
+        assert (k > 0) by nia. (*a hint for nia - without it, the following replace will not work *)
+        replace (start + S offset + (S l - S offset) - start) with (S l) in H by nia.
+        replace (start + S offset - start) with (S offset) in H by lia.
+
+        rewrite encodeSubstringInLine'_stepindex_monotone with (index2 := l) in H; [ | lia].
+        eapply encodesPredicateAt_extensional; [ | apply H]. clear H.
+        intros. cbn. split.
+        * intros ((k0 & H2 & H3) & H4). split; [ | easy]. 
+          destruct k0; [ now left | right]. 
+          split; [ | rewrite projVars_length; [ easy | nia] ]. 
+          exists (k0). split; [ easy | ]. 
+          rewrite projVars_comp. 
+          cbn [Nat.mul] in H3.  
+          enough (|s| <= l - offset - k0 * S offset).
+          { rewrite Nat.min_l by lia. rewrite Nat.add_comm. apply H3. }
+          apply projVars_in_ge in H3; nia.
+        * intros (H & H2). split; [ | apply H2]. 
+          destruct H as [H | (H & _)]; [ exists 0; cbn; easy | ]. 
+          destruct H as (k0 & H & H'). 
+          exists (S k0). split; [ nia | ].
+          rewrite projVars_comp in H'. 
+
+          enough (|s| <= l - offset - k0 * S offset).
+          { rewrite Nat.min_l in H' by lia. cbn [Nat.mul]. rewrite <- Nat.add_comm. apply H'. }
+          apply list_eq_length in H'. 
+          match type of H' with (|projVars ?a ?b ?c| = _) => specialize (projVars_length_le2 a b c) as H3 end.
+          lia. 
+    + (*the case where the remaining string is too short in order to place the substring constraint *)
+      clear IH. assert ( (S l) < (|s|)) as H3%Nat.ltb_lt by lia. cbn -[projVars]; setoid_rewrite H3.
+      split; [eauto | ]. unfold satisfies; cbn [negb evalFormula]. setoid_rewrite explicitAssignment_length. 
+      intros a; split; [congruence | ]. 
+      intros ((k & H1 & H2) & _). 
+      apply list_eq_length in H2. specialize (projVars_length_le (k * offset) (|s|) (explicitAssignment a start (S l))) as H4.
+      rewrite explicitAssignment_length in H4. lia. 
+  Qed.
+
+  (*TODO: consistent argument order over all functions *)
+  Definition encodeSubstringInLine s start l := encodeSubstringInLine' s l l start. 
+  Definition encodeFinalConstraint (start : nat) := listOr (map (fun s => encodeSubstringInLine s start llength) final). 
+
+  Lemma encodesPredicate_listOr (X : Type) (l : list X) (encode : X -> nat -> nat -> formula) (p : X -> list bool -> Prop) start len : 
+    (forall x, x el l -> encodesPredicateAt start len (encode x start len) (p x)) 
+   -> encodesPredicateAt start len (listOr (map (fun x => encode x start len) l)) (fun m => (exists x, x el l /\ p x m) /\ |m| = len). 
+  Proof. 
+    intros H. induction l. 
+    - cbn. split; [easy | ]. unfold satisfies; cbn. intros a; split; [ congruence | intros ((_ & [] & _) & _)]. 
+    - specialize (IHl (fun x Hel => H x (or_intror Hel))). cbn. 
+      specialize (H a (or_introl eq_refl)). 
+      specialize (encodesPredicate_or H IHl) as H1. clear IHl H. 
+      encodesPredicateAt_comp_simp H1. 
+      replace (start + len - start) with len in H1 by lia. 
+
+      eapply encodesPredicateAt_extensional; [ clear H1| apply H1].
+      intros; split.
+      + intros ((x & [-> | H] & H1) & H2); (split; [ | easy]). 
+        * left; now rewrite projVars_all.
+        * right. rewrite projVars_length, projVars_all; easy. 
+      + intros ([H | ((x & H & H') & H1)] & H2); (split; [ | easy]).
+        * exists a. now rewrite projVars_all in H.
+        * exists x. rewrite projVars_length in H1; [ | easy]. rewrite projVars_all in H'; easy.
+  Qed. 
+
+  Lemma encodeFinalConstraint_encodesPredicate start : encodesPredicateAt start llength (encodeFinalConstraint start) (fun m => satFinal offset llength final m /\ |m| = llength).
+  Proof. 
+    unfold encodeFinalConstraint. 
+    eapply encodesPredicateAt_extensional; [ | apply encodesPredicate_listOr]. 
+    2: { intros. apply encodeSubstringInLine'_encodesPredicate; [easy | apply A]. }
+    intros. split. 
+    - intros ((subs & k & H1 & H2 & H3) & H4). split; [ | easy].
+      exists subs. split; [ apply H1 | split; [ | apply H4]]. 
+      exists k. split; [ easy | ]. 
+      destruct H3 as (b & H3). unfold projVars. rewrite H3. 
+      rewrite firstn_app, firstn_all, Nat.sub_diag; cbn. now rewrite app_nil_r. 
+    - intros ((subs & H1 & (k & H2 & H3) & H4) & _). split; [ | apply H4].
+      exists subs, k. split; [apply H1 | split; [ apply H2 | ]].
+      unfold prefix. unfold projVars in H3. 
+      setoid_rewrite <- firstn_skipn with (l := skipn (k * offset) m) (n:= |subs|).
+      setoid_rewrite H3. eauto.
+  Qed. 
+
+  Definition encodeTableau := encodeListAt 0 init ∧ encodeWindowsInAllLines ∧ encodeFinalConstraint (steps * llength).
+  Lemma encodeTableau_encodesPredicate : 
+    encodesPredicateAt 0 (S steps * llength) encodeTableau 
+    (fun m => projVars 0 llength m = init 
+      /\ (forall i, 0 <= i < steps -> valid offset width windows (projVars (i * llength) llength m) (projVars (S i * llength) llength m)) 
+      /\ satFinal offset llength final (projVars (steps * llength) llength m)
+      /\ |m| = (S steps * llength)). 
+  Proof. 
+    specialize (encodesPredicate_and (encodeListAt_encodesPredicate 0 init) encodeWindowsInAllLines_encodesPredicate) as H. 
+    encodesPredicateAt_comp_simp H.  
+    specialize (encodesPredicate_and H (encodeFinalConstraint_encodesPredicate (steps * llength))) as H1.
+    clear H. 
+    encodesPredicateAt_comp_simp H1. 
+    unfold encodeTableau. 
+    replace (llength + steps * llength - 0 - 0) with (S steps * llength) in H1 by lia.
+
+    eapply encodesPredicateAt_extensional; [ clear H1| apply H1].
+    intros m; cbn. rewrite !projVars_comp. setoid_rewrite projVars_comp.
+    rewrite !Nat.min_l by nia. cbn. 
+    setoid_rewrite Nat.add_0_r. setoid_rewrite Nat.sub_0_r. 
+    split. 
+    - intros (H1 & H2 & H3 & H4). 
+      repeat split; try (rewrite projVars_length; nia); try nia; [easy | | easy].
+      intros. rewrite !Nat.min_l by nia. now apply H2.
+    - rewrite !and_assoc. intros (H1 & H2 & (_ & _ & H3 & _ & H4)); split; [easy |split;[ | easy]]. 
+      intros. specialize (H2 i H). rewrite !Nat.min_l in H2 by nia. apply H2.
+  Qed. 
+
+  Lemma expAssgn_to_assgn s b : 
+    {a & forall x, x el a <-> x >= s /\ nth_error b (x - s) = Some true}.
+  Proof. 
+    revert s. 
+    induction b; cbn; intros. 
+    - exists []. intros x. destruct (x-s); cbn; easy. 
+    - destruct (IHb (S s)) as (assgn & IH). destruct a. 
+      + exists (s :: assgn). intros x. split.
+        * intros [-> | H]; [ rewrite Nat.sub_diag; easy | ]. 
+          apply IH in H as (H1 & H2). split; [ lia | ]. 
+          now eapply nth_error_step.
+        * intros (H1 & H2). apply le_lt_eq_dec in H1 as [H1 | ->].
+          -- right. apply IH. split; [ lia | ]. eapply nth_error_step, H2. lia. 
+          -- now left. 
+      + exists assgn. intros x. split.
+        * intros (H1 & H2)%IH. split; [ lia | rewrite <- nth_error_step; easy]. 
+        * intros (H1 & H2). apply le_lt_eq_dec in H1 as [H1 | ->]. 
+          -- apply IH. split; [ lia | ]. apply nth_error_step in H2; easy.  
+          -- rewrite Nat.sub_diag in H2. cbn in H2. congruence. 
+  Qed. 
+
+  Lemma expAssgn_to_assgn_inv a s b : (forall x, x el a <-> x >= s /\ nth_error b (x -s) = Some true) 
+    -> explicitAssignment a s (|b|) = b. 
+  Proof. 
+    revert s. induction b; cbn; intros; [ easy | ].
+    destruct list_in_decb eqn:H1. 
+    - apply list_in_decb_iff in H1; [ | intros; now rewrite Nat.eqb_eq]. 
   Admitted. 
 
+  Lemma relpower_valid_to_assignment n x y: 
+    relpower (valid offset width windows) n x y -> |x| = llength 
+    -> exists m, |m| = (S n * llength) /\ projVars 0 llength m = x /\ projVars (n * llength) llength m = y 
+      /\ (forall i, 0 <= i < n -> valid offset width windows (projVars (i * llength) llength m) (projVars (S i * llength) llength m)). 
+  Proof. 
+    induction 1. 
+    - cbn. exists a. rewrite projVars_all; [ | lia]. easy.
+    - intros. specialize (valid_length_inv H) as H2. rewrite H1 in H2; symmetry in H2. 
+      apply IHrelpower in H2 as (m & H2 & H3 & H4 & H5). clear IHrelpower. 
+      exists (a ++ m). repeat split. 
+      + rewrite app_length. lia. 
+      + rewrite projVars_app1; easy. 
+      + cbn. rewrite projVars_app3; easy.
+      + intros i H6. destruct i. 
+        * cbn. rewrite Nat.add_0_r. setoid_rewrite projVars_app2 at 2; [ | easy]. 
+          rewrite !projVars_app1; [ | easy]. rewrite H3. apply H.
+        * assert (0 <= i < n) as H7 by lia. apply H5 in H7; clear H5 H6. 
+          cbn. rewrite !projVars_app3; [ | easy | easy].  apply H7.
+  Qed. 
+  
   Lemma reduction_wf : FSAT encodeTableau <-> exists sf, relpower (valid offset width windows) steps init sf /\ satFinal offset llength final sf. 
-  Proof. 
-  Admitted. 
+  Proof with (try (solve [rewrite explicitAssignment_length; cbn; nia | cbn; lia])). 
+    specialize (encodeTableau_encodesPredicate) as (H1 & H2). split; intros. 
+    - destruct H as (a & H). apply H2 in H as (H3 & H4 & H5). clear H2. rewrite Nat.add_0_r in *. 
+      exists (projVars (steps * llength) llength (explicitAssignment a 0 (S steps * llength))). 
+      split; [ | apply H5]. rewrite <- H3. clear H1 H3 H5. 
+
+      cbn. rewrite projVars_length... rewrite explicitAssignment_app at 1... rewrite projVars_app1...
+      rewrite Nat.add_comm. rewrite explicitAssignment_app, projVars_app2, projVars_all... 
+
+      apply relpower_relpowerRev. induction steps. 
+      + cbn. constructor. 
+      + econstructor. 
+        * apply IHn. intros. specialize (H4 i). clear IHn. 
+          replace (S (S n) * llength) with (i * llength + (llength + (S n - i) * llength)) in H4 at 1 by nia. 
+          replace (S (S n) * llength) with (S i * llength + (llength + (n - i) * llength)) in H4 by nia. 
+          rewrite explicitAssignment_app, projVars_app2 in H4...
+          rewrite explicitAssignment_app, projVars_app1 in H4...
+          rewrite explicitAssignment_app, projVars_app2 in H4...
+          rewrite explicitAssignment_app, projVars_app1 in H4...
+          
+          replace (S n * llength) with (i * llength + (llength + (n - i) * llength)) at 1 by nia. 
+          replace (S n * llength) with (S i * llength + (llength + (n - S i) * llength)) by nia. 
+          rewrite explicitAssignment_app, projVars_app2...
+          rewrite explicitAssignment_app, projVars_app1...
+          rewrite explicitAssignment_app, projVars_app2...
+          rewrite explicitAssignment_app, projVars_app1...
+          now apply H4. 
+        * specialize (H4 n). clear IHn. 
+          cbn in H4. rewrite Nat.add_comm in H4. setoid_rewrite Nat.add_comm in H4 at 2. setoid_rewrite <- Nat.add_assoc in H4 at 1.
+          rewrite explicitAssignment_app, projVars_app2 in H4... cbn in H4. 
+          rewrite explicitAssignment_app, projVars_app1 in H4... 
+          rewrite explicitAssignment_app, projVars_app2, projVars_all in H4... cbn in H4. now apply H4. 
+    - destruct H as (sf & H3 & H4). unfold encodeTableau in *. 
+      specialize (relpower_valid_to_assignment H3 eq_refl) as (expAssgn & H5 & H6 & H7 & H8). 
+      destruct (expAssgn_to_assgn 0 expAssgn) as (a & H9).
+      exists a. apply H2. clear H2. 
+      apply expAssgn_to_assgn_inv in H9. rewrite H5 in H9. rewrite H9. easy.
+  Qed. 
+
 
 End fixInstance.
 
